\documentclass{article}
\input{503macros.tex}
\def\unityid{rsandil}

\begin{document}
\begin{center}
  {\LARGE CSC 503 Homework Assignment 5}\\[1pc]
  Out: September 11, 2015 \\
  Due: September 18, 2015 \\
  \unityid
\end{center}

In using the Fitch macros to typeset proofs in first order logic, one
introduces a dummy variable $x$ by means of the command
\verb+\open[x]+. 

\begin{enumerate}

\item {[10 points]} Using only the basic natural deduction rules, find
  a proof for
  \begin{displaymath}
    \forall x (P(x) \implies Q(x)) \turn \forall x P(x) \implies
    \forall x Q(x).
\end{displaymath}
\begin{answer}
	\[
		\begin{nd}
			\hypo{1} {\forall x (P(x) \implies Q(x)))} \premise{}
			\open
			\hypo{2} {\forall x (P(x)} \assumption{}
			\open[x_0]
			\have{3}{(P(x_0) \implies Q(x_0))} \Ae {1}
			\have{4}{P(x_0)} \Ae{2}
			\have{5}{Q(x_0)} \ie {3, 4}			
			\close
			\have{6}{\forall x Q(x)} \Ai {3-5}
			\close
			\have{7}{\forall x P(x) \implies \forall x Q(x)} \ii {2-6}
			

		\end{nd}
	\]
\end{answer}
\item {[20 points]} Using only the basic natural deduction rules, find
  a proof for
  \begin{displaymath}
    \forall x \forall y P(x,y) \turn \forall u \forall v P(u,v).
\end{displaymath}
\begin{answer}
	\[
		\begin{nd}
			\hypo{1} {\forall x \forall y P(x,y)} \premise{}
			\open[x_0]
			\have{2} { \forall y P(x_0,y)} \Ae {1}
            \open[y_0]
			\have{3} { P(x_0,y_0)}      \Ae {2}
			\close
			\have{4} {\forall v P(x_0,v)}      \Ai {3}
			\close
			\have{5} {\forall u \forall v P(u,v)}   \Ai {2-4}
			
			
			

		\end{nd}
	\]
\end{answer}

\item {[35 points]} Using only the basic natural deduction rules, find
  a proof for
  \begin{displaymath}
    \exists x (\neg P(x) \lor Q(x)) \turn \exists x \neg (P(x) \land
    \neg Q(x)).
\end{displaymath}
\begin{answer}
	\[
		\begin{nd}
			\hypo{1} {\exists x (\neg P(x) \lor Q(x))} \premise{}
			\open[x_0]
				\have{2} {\neg P(x_0) \lor Q(x_0)} \Ee {1}
				\hypo{3} {P(x_0)\land \neg Q(x_0)} \assumption{}
				\open
					\hypo{4} {\neg P(x_0)} \assumption{}
					\have{5} {P(x_0)} \aeone {3}
					\have{6} {\bot} \ne {5,4}
				\close
				\open
					\hypo{7} {Q(x_0)} \assumption{}
					\have{8} {\neg Q(x_0)} \aetwo {3}
					\have{9} {\bot} \ne {8,7}
				\close				
				\have{10} {\neg(P(x_0)\land \neg Q(x_0))} \ni {3, 4-6,7-9}
			\close
			\have{11} {\exists x \neg(P(x_0)\land \neg Q(x_0))} \Ei {2-10}
		\end{nd}
	\]

\end{answer}
\item {[35 points]} Using only the basic natural deduction rules, find
  a proof for
  \begin{displaymath}
    \forall x \forall y \forall z [S(x,y) \land S(y,z) \implies
    S(x,z)],
    \forall x \neg S(x,x)
    \turn
    \forall x \forall y [S(x,y) \implies (\neg S(y,x) \lor S(x,x))]
\end{displaymath}
\begin{answer}
	\[
		\begin{nd}
		\hypo{1} {\forall x \forall y \forall z [S(x,y) \land S(y,z) \implies S(x,z)]} \premise{}
		\hypo{2} {\forall x \neg S(x,x)} \premise{}
		\open[x_0]
		\have{3} {\neg S(x_0,x_0)} \Ae {2}
		\have{4} {\forall y \forall z [S(x_0,y) \land S(y,z) \implies S(x_0,z)]} \Ae {1}
		\have{5} {\forall y [S(x_0,y) \land S(y,x_0) \implies S(x_0,x_0)]} \Ae {4}
		\open[y_0]
		\have{6} {S(x_0,y_0) \land S(y_0,x_0) \implies S(x_0,x_0)} \Ae {5}
		\open
		\hypo{7} {S(x_0,y_0)} \assumption{}
		\open
		\hypo{8} {S(y_0,x_0)} \assumption{}
		\have{9} {S(x_0,y_0) \land S(y_0,x_0)} \ai {7,8}
		\have{10} {S(x_0,x_0)} \ie {6,9}
		\have{11}  \bot        \ni {3, 10}
		\close
		\have{12} {\neg S(y_0,x_0)} \ni {8-11}
		\have{13} {\neg S(y_0,x_0) \lor S(x_0,x_0)} \oi {12}
		\close
		\have{14} {S(x_0,y_0) \implies \neg S(y_0,x_0) \lor S(x_0,x_0)} \ii {7-13}
		\close
		\have{15} {\forall y[S(x_0,y) \implies \neg S(y,x_0) \lor S(x_0,x_0)]} \Ai {6-14}
		\close
		\have{16} {\forall x \forall y[S(x,y) \implies \neg S(y,x) \lor S(x,x)]} \Ai {3-15}
		\end{nd}
	\]
\end{answer}
\end{enumerate}
\end{document}
